proof/iu_system/uni/decl_worklist/def.v
@@ -13,7 +13,7 @@ Fixpoint dwl_app (Ω1 Ω2 : dworklist) :=
   | dworklist_conswork Ω1' w => dworklist_conswork (dwl_app Ω1' Ω2) w
   end.
 
-(* TODO : check *)
+(* TODO : could change to cont -> typ -> work *)
 Inductive d_apply_cont : cont -> typ -> dworklist -> Prop :=
   (* | d_applycont__done : forall T1,  
       d_apply_cont cont_done (some T1) dworklist_empty *)
